Add Coq interpreter for Checked.t

coq/checked.v
@@ -1,22 +1,38 @@
+Require Import String.
+Require Import List.
+Import List.ListNotations.
+Require Import String.
 Require Import Snarky.monad.
-Require Snarky.types.
+Require Import Snarky.types.
+Require Snarky.field.
+Require Snarky.cvar.
+Require Snarky.as_prover.
+Require Snarky.R1CS_constraint_system.
+Require Snarky.constraint.
+Require Snarky.provider.
+Require Snarky.typ_monads.
+Require Snarky.backend.
 Export Snarky.types.Checked.
 Export Snarky.types.Types.
+
+Set Universe Polymorphism.
 
 Section Instances.
 
   Variables F V sys S : Type.
+  Variable req : Type -> Type.
 
-  Global Instance checked_return : Return (t F V sys S) := {
+  Global Instance checked_return : Return (t F V sys req S) := {
     ret A x := Pure x
   }.
 
-  Global Instance checked_map : Map (t F V sys S) := {
+  Global Instance checked_map : Map (t F V sys req S) := {
     map :=
-      (fix map' S A B (t : checked F V sys S A) : (A -> B) -> checked F V sys S B :=
-        match t in checked _ _ _ s a return (a -> B) -> checked F V sys s B with
+      (fix map' S A B (t : checked F V sys req S A) : (A -> B) -> checked F V sys req S B :=
+        match t in checked _ _ _ _ s a return (a -> B) -> checked F V sys req s B with
         | Pure x => fun f => Pure (f x)
         | With_label s t k => fun f => With_label s t (fun b => map' _ _ _ (k b) f)
+        | With_constraint_system c k => fun f => With_constraint_system c (map' _ _ _ k f)
         | As_prover x k => fun f => As_prover x (map' _ _ _ k f)
         | Add_constraint c t1 => fun f => Add_constraint c (map' _ _ _ t1 f)
         | With_state p and_then t_sub k =>
@@ -28,12 +44,13 @@ Section Instances.
         end) S
   }.
 
-  Global Instance checked_bind : Bind (t F V sys S) := {
+  Global Instance checked_bind : Bind (t F V sys req S) := {
     bind :=
-      (fix bind' S A B (t : checked F V sys S A) : (A -> checked F V sys S B) -> checked F V sys S B :=
-        match t in checked _ _ _ s a return (a -> checked F V sys s B) -> checked F V sys s B with
+      (fix bind' S A B (t : checked F V sys req S A) : (A -> checked F V sys req S B) -> checked F V sys req S B :=
+        match t in checked _ _ _ _ s a return (a -> checked F V sys req s B) -> checked F V sys req s B with
         | Pure x => fun f => f x
         | With_label s t k => fun f => With_label s t (fun b => bind' _ _ _ (k b) f)
+        | With_constraint_system c k => fun f => With_constraint_system c (bind' _ _ _ k f)
         | As_prover x k => fun f => As_prover x (bind' _ _ _ k f)
         | Add_constraint c t1 => fun f => Add_constraint c (bind' _ _ _ t1 f)
         | With_state p and_then t_sub k =>
@@ -47,4 +64,270 @@ Section Instances.
 
 End Instances.
 
-Definition as_prover {F V sys S} x : t F V sys S unit := As_prover x ((ret : _ -> t _ _ _ _ _) tt).
+Definition as_prover {F V sys req S} x : t F V sys req S unit :=
+  As_prover x ((ret : _ -> t _ _ _ _ _ _) tt).
+
+Module Run.
+  Section Run_util.
+    Set Implicit Arguments.
+    Record run_state (F sys' : Type) (req : Type -> Type) (S : Type) :=
+    { num_inputs : nat
+    ; input : list F
+    ; next_auxiliary : nat
+    ; aux : list F
+    ; system : option (backend.R1CS_constraint_system.t sys')
+    ; eval_constraints : bool
+    ; handler : request.Handler.t req
+    ; state : option S
+    ; stack : list string }.
+    Unset Implicit Arguments.
+
+    Context {F sys' : Type} {req : Type -> Type} `{field.Field F}.
+
+    Definition sys := backend.R1CS_constraint_system.t sys'.
+
+    Definition var := types.Cvar.t F nat.
+
+(*Definition run {F sys S A} `{field.Field F} (num_inputs : nat) (input : list F) (aux : list F) (system : option sys)
+  (eval_constraints : bool) (t0 : t F nat sys S A) (s0 : option s) :=
+  let next_auxiliary := 1 + num_inputs in
+  let eval_constraints := match s0 with
+    | Some _ => eval_constraints
+    | None => false
+    end in
+  let get_value := get_value num_inputs input in
+  let run_as_prover := run_as_prover num_inputs input in
+  let system := match system with
+    | Some system => Some (R1CS_constraint_system.set_primary_input_size system num_inputs)
+    | None => None in*)
+
+    Definition set_next_auxiliary {S : Type} (next_auxiliary : nat) (run_state : run_state F sys' req S) :=
+    {| num_inputs := num_inputs run_state
+    ; input := input run_state
+    ; next_auxiliary := next_auxiliary
+    ; aux := aux run_state
+    ; system := system run_state
+    ; eval_constraints := eval_constraints run_state
+    ; handler := handler run_state
+    ; state := state run_state
+    ; stack := stack run_state |}.
+
+    Definition set_aux {S : Type} (aux : list F) (run_state : run_state F sys' req S) :=
+    {| num_inputs := num_inputs run_state
+    ; input := input run_state
+    ; next_auxiliary := next_auxiliary run_state
+    ; aux := aux
+    ; system := system run_state
+    ; eval_constraints := eval_constraints run_state
+    ; handler := handler run_state
+    ; state := state run_state
+    ; stack := stack run_state |}.
+
+    Definition set_system {S : Type} (system : option sys) (run_state : run_state F sys' req S)
+      : Run_util.run_state F sys' req S :=
+    {| num_inputs := num_inputs run_state
+    ; input := input run_state
+    ; next_auxiliary := next_auxiliary run_state
+    ; aux := aux run_state
+    ; system := system
+    ; eval_constraints := eval_constraints run_state
+    ; handler := handler run_state
+    ; state := state run_state
+    ; stack := stack run_state |}.
+
+    Definition set_handler {S : Type} (handler : request.Handler.t req)
+      (run_state : run_state F sys' req S) :=
+    {| num_inputs := num_inputs run_state
+    ; input := input run_state
+    ; next_auxiliary := next_auxiliary run_state
+    ; aux := aux run_state
+    ; system := system run_state
+    ; eval_constraints := eval_constraints run_state
+    ; handler := handler
+    ; state := state run_state
+    ; stack := stack run_state |}.
+
+    Definition set_state {S1 S2 : Type} (state : option S2) (run_state : run_state F sys' req S1) :=
+    {| num_inputs := num_inputs run_state
+    ; input := input run_state
+    ; next_auxiliary := next_auxiliary run_state
+    ; aux := aux run_state
+    ; system := system run_state
+    ; eval_constraints := eval_constraints run_state
+    ; handler := handler run_state
+    ; state := state
+    ; stack := stack run_state |}.
+
+    Definition set_stack {S : Type} (stack : list string)
+      (run_state : run_state F sys' req S) :=
+    {| num_inputs := num_inputs run_state
+    ; input := input run_state
+    ; next_auxiliary := next_auxiliary run_state
+    ; aux := aux run_state
+    ; system := system run_state
+    ; eval_constraints := eval_constraints run_state
+    ; handler := handler run_state
+    ; state := state run_state
+    ; stack := stack |}.
+
+    Definition get_value {S : Type} (rstate : run_state F sys' req S) : var -> F :=
+      let num_inputs := num_inputs rstate in
+      let get_one i :=
+        if Compare_dec.le_lt_dec i num_inputs then
+          List.nth (i - 1) (input rstate) field.zero
+        else
+          List.nth (i - num_inputs - 1) (aux rstate) field.zero in
+      cvar.eval get_one.
+
+    Definition store_field_elt {S : Type} (rstate : run_state F sys' req S) x
+      : run_state F sys' req S * var :=
+     let v := next_auxiliary rstate in
+     let rstate := set_aux (aux rstate ++ [x]) rstate in
+     let rstate := set_next_auxiliary (v + 1) rstate in
+     (rstate, cvar.Unsafe.of_var v).
+
+    Definition alloc_var {S : Type} (rstate : run_state F sys' req S) :
+      run_state F sys' req S * var :=
+      let v := next_auxiliary rstate in
+      let rstate := set_next_auxiliary (v + 1) rstate in
+      (rstate, cvar.Unsafe.of_var v).
+
+    Definition run_as_prover {S S' A : Type} (rstate : run_state F sys' req S')
+      (x : option (as_prover.t F var S A)) (s : option S) : option S * option A :=
+      match x, s with
+      | Some x, Some s =>
+        let (s', y) := as_prover.run x (get_value rstate) s in
+        (Some s', Some y)
+      | _, _ => (None, None)
+      end.
+
+  Context {linear_combination constraint : Type}.
+  Context `{backend.R1CS_constraint_system F constraint sys'}.
+  Context `{backend.R1CS_constraint constraint linear_combination}.
+  Context `{backend.R1CS_constraint}.
+  Context `{backend.Linear_combination linear_combination F (cvar.t F nat)}.
+
+  Definition add_constraint {S : Type} (c : types.Constraint.t var)
+    (rstate : run_state F sys' req S) : run_state F sys' req S :=
+    match system rstate with
+    | Some system =>
+      let stack := stack rstate in
+      set_system (Some (constraint.add stack c system)) rstate
+    | None => rstate
+    end.
+
+  Definition store_or_alloc {Var Value S} (typ : Typ.t F var sys req Var Value)
+    (value : option Value) (rstate : run_state F sys' req S) :=
+    match value with
+    | Some value =>
+      typ_monads.Store.run (Typ.store typ value) store_field_elt rstate
+    | None => typ_monads.Alloc.run (Typ.alloc typ) alloc_var rstate
+    end.
+  End Run_util.
+
+  Section Run_aux.
+    Context {F sys' : Type} {req : Type -> Type} `{field.Field F}.
+
+    Context {linear_combination constraint : Type}.
+    Context `{backend.R1CS_constraint_system F constraint sys'}.
+    Context `{backend.R1CS_constraint constraint linear_combination}.
+    Context `{backend.R1CS_constraint}.
+    Context `{backend.Linear_combination linear_combination F (cvar.t F nat)}.
+
+    Fixpoint run_aux {S A : Type} (rstate : run_state F sys' req S) (t : t F var sys req S A)
+      {struct t} : (run_state F sys' req S * A) + _ :=
+      match t in types.Types.checked _ _ _ _ s a
+      return run_state F sys' req s -> (run_state F sys' req s * a) + _ with
+      | Pure x => fun rstate => inl (rstate, x)
+      | With_constraint_system f k => fun rstate =>
+        let system := match system rstate with
+          | Some system => Some (f system)
+          | None => None
+          end in
+        run_aux (set_system system rstate) k
+      | With_label lab t k => fun rstate =>
+        let stack := stack rstate in
+        match run_aux (set_stack (lab :: stack) rstate) t with
+        | inl (rstate, y) => run_aux (set_stack stack rstate) (k y)
+        | inr err => inr err
+        end
+      | As_prover x k => fun rstate =>
+        let (s, _) := run_as_prover rstate (Some x) (state rstate) in
+        run_aux (set_state s rstate) k
+      | Add_constraint c t1 => fun rstate =>
+        (** TODO: currently ignoring this. *)
+        let failed := andb (eval_constraints rstate) (constraint.eval c (get_value rstate)) in
+        if failed then
+          inr (String.concat "\n" ["Constraint unsatisfied:"; constraint.annotation c;
+            constraint.stack_to_string (stack rstate)]%string)
+        else run_aux (add_constraint c rstate) t1
+      | With_state p and_then t_sub k => fun rstate =>
+        let s := state rstate in
+        let (s1, s_sub) := run_as_prover rstate (Some p) s in
+        match run_aux (set_state s_sub rstate) t_sub with
+        | inl (rstate, y) =>
+          let p1 := match state rstate return forall T, (_ -> T) -> option T with
+            | Some s_sub => fun T and_then => Some (and_then s_sub)
+            | None => fun _ _ => None
+            end _ and_then in
+          let rstate := set_state s rstate in
+          let (s, _) := run_as_prover rstate p1 s1 in
+          run_aux rstate (k y)
+        | inr err => inr err
+        end
+      | With_handler h t k => fun rstate =>
+        let handler := handler rstate in
+        let rstate := set_handler (request.Handler.push handler h) rstate in
+        match run_aux rstate t with
+        | inl (rstate, y) => run_aux (set_handler handler rstate) (k y)
+        | inr err => inr err
+        end
+      | Clear_handler t k => fun rstate =>
+        let handler := handler rstate in
+        let rstate := set_handler (List.nil) rstate in
+        match run_aux rstate t with
+        | inl (rstate, y) => run_aux (set_handler handler rstate) (k y)
+        | inr err => inr err
+        end
+      | Next_auxiliary k => fun rstate =>
+        run_aux rstate (k (next_auxiliary rstate))
+      | Exists typ p k => fun rstate =>
+        match state rstate with
+        | Some s =>
+          let (s', value) := provider.run p (get_value rstate) s (handler rstate) in
+          match value with
+          | Some value =>
+            let (rstate, var) := typ_monads.Store.run (Typ.store typ value) store_field_elt rstate in
+            match run_aux (set_state (Some tt) rstate) (Typ.check typ var) with
+            | inl (rstate, _) =>
+              run_aux (set_state (Some s') rstate)
+                (k {| Handle.var := var; Handle.value := Some value |})
+            | inr err => inr err
+            end
+          | None => inr "Unhandled request"%string
+          end
+        | None => 
+          let (rstate, var) := typ_monads.Alloc.run (Typ.alloc typ) alloc_var rstate in
+          match run_aux (set_state None rstate) (Typ.check typ var) with
+          | inl (rstate, _) =>
+            run_aux (set_state None rstate) (k {| Handle.var := var; Handle.value := None |})
+          | inr err => inr err
+          end
+        end
+      end rstate.
+
+  Definition run {A S} (input : list F) (system : option sys) (eval_constraints : bool)
+    (t : t F var sys req S A) (s : option S) :=
+    let num_inputs := List.length input in
+    let rstate := {|
+      num_inputs := num_inputs
+    ; input := input
+    ; next_auxiliary := num_inputs + 1
+    ; aux := []
+    ; system := system
+    ; eval_constraints := eval_constraints
+    ; handler := request.Handler.fail
+    ; state := s
+    ; stack := []
+    |} in
+    run_aux rstate t.
