coq/types.v
@@ -1,5 +1,7 @@
 Require Import String.
 Require Import Snarky.typ_monads.
+Require Snarky.request.
+Require Utils.
 
 Module Constraint.
   Module Basic.
@@ -8,11 +10,20 @@ Module Constraint.
       | Equal : var -> var -> t var
       | Square : var -> var -> t var
       | R1CS : var -> var -> var -> t var.
+
+
+    Arguments Boolean {var}.
+    Arguments Equal {var}.
+    Arguments Square {var}.
+    Arguments R1CS {var}.
   End Basic.
 
   Record basic_with_annotation var : Type := {
-    basic : Basic.t var; annotation : option string
+    basic : Basic.t var; annot : option string
   }.
+
+  Arguments basic {var}.
+  Arguments annot {var}.
 
   Definition t var := list (basic_with_annotation var).
 End Constraint.
@@ -23,27 +34,47 @@ Module Cvar.
   | Var : v -> t f v
   | Add : t f v -> t f v -> t f v
   | Scale : f -> t f v -> t f v.
+
+  Arguments Constant {f v}.
+  Arguments Var {f v}.
+  Arguments Add {f v}.
+  Arguments Scale {f v}.
 End Cvar.
 
 Module As_prover.
   Definition t f v s a := (v -> f) -> s -> s * a.
 End As_prover.
 
-Parameter request_handler : Type.
+Module Provider.
+  Inductive t F V S request A :=
+    | Request : As_prover.t F V S (request A) -> t F V S request A
+    | Compute : As_prover.t F V S A -> t F V S request A
+    | Both : As_prover.t F V S (request A) -> As_prover.t F V S A -> t F V S request A.
 
-Parameter provider : forall (a env s : Type), Type.
+  Arguments Request {F V S request A}.
+  Arguments Compute {F V S request A}.
+  Arguments Both {F V S request A}.
+End Provider.
 
-Parameter handle : forall (var value : Type), Type.
+Module Handle.
+
+  Inductive t var value := {var : var; value : option value}.
+
+End Handle.
 
 Module Types.
   Section type.
     Polymorphic Variables f v sys : Type.
+    Polymorphic Variable request : Type -> Type.
 
     Polymorphic Inductive checked : forall (s a : Type), Type :=
       | Pure a s : a -> checked s a
-      | Add_constraint a s : Constraint.t v -> checked s a -> checked s a
+      | Add_constraint a s :
+          Constraint.t v -> checked s a -> checked s a
+      | With_constraint_system a s :
+          (sys -> sys) -> checked s a -> checked s a
       | As_prover a s :
-          As_prover.t f v sys unit ->
+          As_prover.t f v s unit ->
           checked s a ->
           checked s a
       | With_label a b s :
@@ -58,7 +89,7 @@ Module Types.
           (b -> checked s1 a) ->
           checked s1 a
       | With_handler a b s :
-          request_handler ->
+          request.Handler.single request ->
           checked s a ->
           (a -> checked s b) ->
           checked s b
@@ -68,8 +99,8 @@ Module Types.
         checked s b
       | Exists a s var value :
         typ var value ->
-        provider value (v -> f) s ->
-        (handle var value -> checked s a) ->
+        Provider.t f v s request value ->
+        (Handle.t var value -> checked s a) ->
         checked s a
       | Next_auxiliary a s :
         (nat -> checked s a) -> checked s a
@@ -83,42 +114,49 @@ Module Types.
           typ var value.
   End type.
 
-  Arguments Pure {f v sys a s}.
-  Arguments Add_constraint {f v sys a s}.
-  Arguments As_prover {f v sys a s}.
-  Arguments With_label {f v sys a b s}.
-  Arguments With_state {f v sys a b s1 s2}.
-  Arguments With_handler {f v sys a b s}.
-  Arguments Clear_handler {f v sys a b s}.
-  Arguments Exists {f v sys a s var value}.
-  Arguments Next_auxiliary {f v sys a s}.
-  Arguments Add_constraint {f v sys a s}.
+  Arguments Pure {f v sys request a s}.
+  Arguments Add_constraint {f v sys request a s}.
+  Arguments With_constraint_system {f v sys request a s}.
+  Arguments As_prover {f v sys request a s}.
+  Arguments With_label {f v sys request a b s}.
+  Arguments With_state {f v sys request a b s1 s2}.
+  Arguments With_handler {f v sys request a b s}.
+  Arguments Clear_handler {f v sys request a b s}.
+  Arguments Exists {f v sys request a s var value}.
+  Arguments Next_auxiliary {f v sys request a s}.
+  Arguments Add_constraint {f v sys request a s}.
 End Types.
 
 Module Checked.
-  Definition t f v sys a s := Types.checked f v sys a s.
+  Definition t := Types.checked.
 End Checked.
 
 Module Typ.
-  Definition t f v sys var value := Types.typ f v sys var value.
+  Definition t := Types.typ.
 
-  Definition store {f v sys var value} (t : t f v sys var value) : value -> Store.t f v var :=
-    match t in Types.typ _ _ _ var value return value -> Store.t f v var with
-    | Types.Mk_typ _ _ _ _ _ store read alloc check => store
-    end.
+  Section Typ.
+    Context {f v sys var value : Type} {request : Type -> Type}.
 
-  Definition read {f v sys var value} (t : t f v sys var value) : var -> Read.t f v value :=
-    match t in Types.typ _ _ _ var value return var -> Read.t f v value with
-    | Types.Mk_typ _ _ _ _ _ store read alloc check => read
-    end.
+    Definition store (t : t f v sys request var value) : value -> Store.t f v var :=
+      match t in Types.typ _ _ _ _ var value return value -> Store.t f v var with
+      | Types.Mk_typ _ _ _ _ _ _ store read alloc check => store
+      end.
 
-  Definition alloc {f v sys var value} (t : t f v sys var value) : Alloc.t v var :=
-    match t in Types.typ _ _ _ var value return Alloc.t v var with
-    | Types.Mk_typ _ _ _ _ _ store read alloc check => alloc
-    end.
+    Definition read (t : t f v sys request var value) : var -> Read.t f v value :=
+      match t in Types.typ _ _ _ _ var value return var -> Read.t f v value with
+      | Types.Mk_typ _ _ _ _ _ _ store read alloc check => read
+      end.
 
-  Definition check {f v sys var value} (t : t f v sys var value) : var -> Checked.t f v sys unit unit :=
-    match t in Types.typ _ _ _ var value return var -> Checked.t f v sys unit unit with
-    | Types.Mk_typ _ _ _ _ _ store read alloc check => check
-    end.
+    Definition alloc (t : t f v sys request var value) : Alloc.t v var :=
+      match t in Types.typ _ _ _ _ var value return Alloc.t v var with
+      | Types.Mk_typ _ _ _ _ _ _ store read alloc check => alloc
+      end.
+
+    Definition check (t : t f v sys request var value)
+      : var -> Checked.t f v sys request unit unit :=
+      match t in Types.typ _ _ _ _ var value
+        return var -> Checked.t f v sys request unit unit with
+      | Types.Mk_typ _ _ _ _ _ _ store read alloc check => check
+      end.
+  End Typ.
 End Typ.
