coq/backend.v
@@ -1,0 +1,88 @@
+Require Snarky.field.
+Require Snarky.bigint.
+Require Snarky.R1CS_constraint_system.
+Require Snarky.cvar.
+
+Module Field := Snarky.field.
+Module Bigint := Snarky.bigint.
+
+Class Field_size (bigint : Type) := { field_size : bigint }.
+
+Module Var.
+  Class Index (t : Type) := { index : t -> nat }.
+  Arguments index {t}.
+
+  Class Create (t : Type) := { create : nat -> t }.
+  Arguments create {t}.
+
+  Class Var (t : Type) :=
+  { var_index :> Index t
+  ; var_create :> Create t
+  }.
+
+  Module Class.
+    Instance nat_var : Var nat :=
+    {| var_index := {| index := fun n => n |}
+    ; var_create := {| create := fun n => n |}
+    |}.
+  End Class.
+  Include Class.
+End Var.
+
+Module Linear_combination.
+  Class Create (t : Type) := { create : unit -> t }.
+  Arguments create {t Create}.
+
+  Class Of_var (t var : Type) := { of_var : var -> t }.
+  Arguments of_var {t var Of_var}.
+
+  Class Of_field (t field : Type) := { of_field : field -> t }.
+  Arguments of_field {t field Of_field}.
+
+  Class Add_term (t field var : Type) := { add_term : t -> field -> var -> t }.
+  Arguments add_term {t field var Add_term}.
+
+  Definition of_constant {t field : Type} `{Create t} `{Of_field t field} c :=
+    match c with
+    | None => create tt
+    | Some c => of_field c
+    end.
+
+  Definition zero {t field A} `{field.Field field A} `{Of_field t field} := of_field field.zero.
+
+  Module Class.
+    Class Linear_combination (t field var : Type) :=
+    { linear_combination_create : Create t
+    ; linear_combination_of_var : Of_var t var
+    ; linear_combination_of_field : Of_field t field
+    ; linear_combination_add_term : Add_term t field var
+    }.
+  End Class.
+  Include Class.
+End Linear_combination.
+
+Module R1CS_constraint. 
+  Class Create (t linear_combination : Type) :=
+    { create : linear_combination -> linear_combination -> linear_combination -> t }.
+  Arguments create {t linear_combination Create}.
+
+  Class Set_is_square (t : Type) := { set_is_square : t -> bool -> t }.
+  Arguments set_is_square {t Set_is_square}.
+
+  Module Class.
+    Class R1CS_constraint (t linear_combination : Type) :=
+    { r1cs_constraint_create :> Create t linear_combination
+    ; r1cs_constraint_set_is_square :> Set_is_square t
+    }.
+  End Class.
+  Include Class.
+End R1CS_constraint.
+
+Module R1CS_constraint_system := R1CS_constraint_system.
+
+Include Field.Class.
+Include Bigint.Class.
+Include Var.Class.
+Include Linear_combination.Class.
+Include R1CS_constraint.Class.
+Include R1CS_constraint_system.Class.
