coq/constraint.v
@@ -1,21 +1,22 @@
+Require Import String.
 Require Snarky.Util.
 Require Import List.
 Import List.ListNotations.
 Require Snarky.types.
+Require Import Snarky.backend.
+Require Snarky.cvar.
 Import Snarky.types.Constraint.Basic.
 Import Snarky.types.Constraint.
 
 Section T.
   Context {V : Type}.
 
-  Definition t := t V.
-
   Definition create_basic label basic : basic_with_annotation V :=
-    {| basic := basic; annotation := label |}.
+    {| basic := basic; annot := label |}.
 
   Definition override_label x label_opt : basic_with_annotation V :=
     {| basic := basic x
-    ; annotation := (match label_opt with Some x => Some x | None => annotation x end) |}.
+    ; annot := (match label_opt with Some x => Some x | None => annot x end) |}.
 
   Definition equal label x y := [create_basic label (Equal x y)].
 
@@ -25,7 +26,72 @@ Section T.
 
   Definition square label a b := [create_basic label (Square a b)].
 
-  Definition annotation (t : t) :=
-    String.concat "; " (Util.List.filter_map annotation t).
+  Definition annotation (t : t V) :=
+    String.concat "; " (Util.List.filter_map annot t).
 
 End T.
+
+Section Snarky.
+
+  Context {field var constraint linear_combination sys A : Type}
+    `{F : Field field A}
+    `{LC : Linear_combination linear_combination field (cvar.t field var)}
+    `{R1C : R1CS_constraint constraint linear_combination}
+    `{R1CS' : R1CS_constraint_system field constraint sys}.
+
+  Definition basic_to_r1cs_constraint (basic : Basic.t (cvar.t field var)) : constraint.
+    destruct LC, R1C.
+    refine (let of_var := Linear_combination.of_var in
+      match basic with
+      | Boolean v =>
+        let lc := of_var v in
+        let constr := R1CS_constraint.create lc lc lc in
+        R1CS_constraint.set_is_square constr true
+      | Equal v1 v2 =>
+        let constr :=
+          R1CS_constraint.create Linear_combination.zero
+            Linear_combination.zero
+            (of_var (cvar.sub v1 v2))
+        in
+        R1CS_constraint.set_is_square constr true
+      | Square a c =>
+        let a := of_var a in
+        let constr := R1CS_constraint.create a a (of_var c) in
+        R1CS_constraint.set_is_square constr true
+      | R1CS a b c =>
+          let constr :=
+            R1CS_constraint.create (of_var a) (of_var b) (of_var c)
+          in
+          R1CS_constraint.set_is_square constr false
+      end); assumption.
+  Defined.
+
+  Definition stack_to_string := String.concat "\n".
+
+  Definition add (stack : list string) (t : t (cvar.t field var))
+    (system : R1CS_constraint_system.t sys) :=
+    List.fold_left (fun system t =>
+      let label := match annot t with
+        | Some label => label
+        | None => ("unknown" : string)%string
+        end in
+      let c := basic_to_r1cs_constraint (basic t) in
+      R1CS_constraint_system.add_constraint_with_annotation system c
+        (stack_to_string (label :: stack)))
+    t system.
+
+  Definition eval_basic (t : Basic.t (cvar.t field var)) get_value :=
+    match t with
+    | Boolean v =>
+      let x := get_value v in
+      orb (field.equal x field.zero) (field.equal x field.one)
+    | Equal v1 v2 => field.equal (get_value v1) (get_value v2)
+    | R1CS v1 v2 v3 =>
+        field.equal (field.mul (get_value v1) (get_value v2)) (get_value v3)
+    | Square a c => field.equal (field.square (get_value a)) (get_value c)
+    end.
+
+  Definition eval (t : t (cvar.t field var)) get_value :=
+     List.forallb (fun t => eval_basic (basic t) get_value) t.
+
+End Snarky.
