coq/request.v
@@ -1,0 +1,39 @@
+Require List.
+
+Module Response.
+  Inductive t (req : Type -> Type) (A : Type) :=
+  | Provide : A -> t req A
+  | Delegate : req A -> t req A
+  | Unhandled : t req A.
+
+  Arguments Provide {req A}.
+  Arguments Delegate {req A}.
+  Arguments Unhandled {req A}.
+End Response.
+
+Module Handler.
+  Import Response.
+
+  Definition single (req : Type -> Type) := forall A, req A -> Response.t req A.
+
+  Definition t req := list (single req).
+
+  Definition fail {req} : t req := List.nil.
+
+  Definition push {req} (t : t req) (single : single req) := cons single t.
+
+  Fixpoint run {req A} (stack : t req) (request : req A) : option A :=
+    match stack with
+    | nil => None
+    | cons handle stack =>
+      match handle _ request with
+      | Provide a => Some a
+      | Delegate request => run stack request
+      | Unhandled => run stack request
+      end
+    end.
+
+  Definition create_single {req} (handler : forall {A}, req A -> Response.t req A)
+    : single req :=
+    @handler.
+End Handler.
