coq/bigint.v
@@ -1,0 +1,31 @@
+Module T.
+  Section T.
+    Class Of_field t F := { of_field : F -> t }.
+    Arguments of_field {t F}.
+
+    Class Test_bit t := { test_bit : t -> nat -> bool }.
+    Arguments test_bit {t}.
+  End T.
+
+End T.
+
+Include T.
+
+Module Class.
+  Class Bigint t F :=
+    { bigint_of_field :> Of_field t F
+    ; bigint_test_bit :> Test_bit t
+    }.
+End Class.
+Include Class.
+
+Module Extended.
+  Include T.
+
+  Section Extended.
+    Context {t F : Type}.
+
+    Class To_field := { to_field : t -> F }.
+
+  End Extended.
+End Extended.
