coq/provider.v
@@ -1,0 +1,24 @@
+Require Snarky.types.
+Require Snarky.as_prover.
+Require Snarky.request.
+
+Include Snarky.types.Provider.
+
+Definition run {F V S request result} (t : t F V S request result) tbl s
+  (handler : request.Handler.t request) :=
+  match t with
+  | Request rc =>
+    let (s', r) := as_prover.run rc tbl s in
+    (s', request.Handler.run handler r)
+  | Compute c =>
+    let (s', r) := as_prover.run c tbl s in
+    (s', Some r)
+  | Both rc c =>
+    let (s', r) := as_prover.run rc tbl s in
+    match request.Handler.run handler r with
+    | Some x => (s', Some x)
+    | None =>
+      let (s', r) := as_prover.run c tbl s in
+      (s', Some r)
+    end
+  end.
